Weidenbach_Book/IsaSAT_Watch_List.thy
@@ -2,12 +2,12 @@ theory IsaSAT_Watch_List
   imports IsaSAT_Clauses
 begin
 
-text \<open>There is not much to say about watch list,s since they are arrays of resizeable arrays,
+text \<open>There is not much to say about watch lists since they are arrays of resizeable arrays,
   which are defined in a separate theory.
 
   However, when replacing the elements in our watch lists from \<^typ>\<open>(nat \<times> uint32)\<close>
   to \<^typ>\<open>(nat \<times> uint32 \<times> bool)\<close>, we got a huge and unexpected slowdown, due to a much higher
-  number of cache misses (roughly 3.5 times as many on a eq.atree.braun.8.unsat.cnf who also took
+  number of cache misses (roughly 3.5 times as many on a eq.atree.braun.8.unsat.cnf which also took
   66s instead of 50s). While toying with the generated ML code, we found out that our version of
   the tuples with booleans were using 40 bytes instead of 24 previously. Just merging the
   \<^typ>\<open>uint32\<close> and the \<^typ>\<open>bool\<close> to a single \<^typ>\<open>uint64\<close> was sufficient to get the
